src/program_proof/wal/circ_proof.v
@@ -560,7 +560,7 @@ Theorem wp_circular__Advance (Q: iProp Σ) γ (d: val) (start0: u64) (newStart :
       diskEnd_at_least γ diskEnd_lb ∗
       ⌜int.Z start0 ≤ int.Z newStart ≤ diskEnd_lb⌝ ∗
     (∀ σ, ⌜circ_wf σ⌝ ∗ P σ ∗ ⌜σ.(circΣ.start) = start0⌝ -∗
-      (∀ σ' b, ⌜relation.denote (circ_advance newStart) σ σ' b⌝ ∗ ⌜circ_wf σ'⌝ ={⊤ ∖↑ N}=∗ P σ' ∗ Q))
+      (∀ σ' b, ⌜relation.denote (circ_advance newStart) σ σ' b⌝ ∗ ⌜circ_wf σ'⌝ -∗ |NC={⊤ ∖↑ N}=> P σ' ∗ Q))
   }}}
     Advance d #newStart
   {{{ RET #(); Q ∗ start_is γ (1/2) newStart }}}.
@@ -1076,7 +1076,7 @@ Theorem wp_circular__Append (Q: iProp Σ) γ (d: val) q (startpos endpos : u64) 
       start_at_least γ startpos ∗
       is_circular_appender γ c ∗
       (∀ σ, ⌜circ_wf σ⌝ ∗ ⌜circΣ.diskEnd σ = int.Z endpos⌝ ∗ P σ -∗
-          ∀ σ' b, ⌜relation.denote (circ_append upds endpos) σ σ' b⌝ ∗ ⌜circ_wf σ'⌝ ={⊤ ∖↑ N}=∗ P σ' ∗ Q)
+          ∀ σ' b, ⌜relation.denote (circ_append upds endpos) σ σ' b⌝ ∗ ⌜circ_wf σ'⌝ -∗ |NC={⊤ ∖↑ N}=> P σ' ∗ Q)
   }}}
     circularAppender__Append #c d #endpos (slice_val bufs)
   {{{ RET #(); Q ∗
