src/program_proof/wal/logger_proof.v
@@ -213,7 +213,7 @@ Proof.
   iMod (ghost_var_update_halves nextDiskEnd_txn_id with "HownLoggerTxn_logger HownLoggerTxn_linv") as
         "[HownLoggerTxn_logger HownLoggerTxn_linv]".
 
-  iAssert (ghost_var γ.(txns_name) (1 / 2) txns ={⊤}=∗ ghost_var γ.(txns_name) (1 / 2) txns ∗ txn_pos γ σ.(locked_diskEnd_txn_id) σ.(diskEnd))%I as "HdiskEnd_pos_helper".
+  iAssert (ghost_var γ.(txns_name) (1 / 2) txns -∗ |NC={⊤}=> ghost_var γ.(txns_name) (1 / 2) txns ∗ txn_pos γ σ.(locked_diskEnd_txn_id) σ.(diskEnd))%I as "HdiskEnd_pos_helper".
   {
     iIntros "Howntxns".
     iDestruct "Hwal" as "[Hwal Hcirc]".
@@ -393,7 +393,7 @@ Proof.
   iDestruct (ghost_var_agree with "HownLoggerPos_linv HownLoggerPos_logger") as %Heqloggerpos; subst.
   iDestruct (ghost_var_agree with "HownLoggerTxn_linv HownLoggerTxn_logger") as %Heqloggertxn; subst.
 
-  iAssert (ghost_var γ.(txns_name) (1 / 2) txns0 ={⊤}=∗
+  iAssert (ghost_var γ.(txns_name) (1 / 2) txns0 -∗ |NC={⊤}=>
            ghost_var γ.(txns_name) (1 / 2) txns0 ∗
            ⌜is_txn txns0 nextDiskEnd_txn_id σ.(memLog).(slidingM.mutable)⌝ ∗
            ⌜subslice (S installed_txn_id_mem) (S nextDiskEnd_txn_id) txns0 =
